![[1 星角变换.png]]
### 星形（Y）到三角形（Δ）变换

$$\begin{gathered}R_{AB}=\frac{R_{A}\cdot R_{B}+R_{B}\cdot R_{C}+R_{C}\cdot R_{A}}{R_{A}+R_{B}+R_{C}}\\R_{BC}=\frac{R_{B}\cdot R_{C}+R_{C}\cdot R_{A}+R_{A}\cdot R_{B}}{R_{A}+R_{E}+R_{C}}\\R_{CA}=\frac{R_{C^{\prime}}R_{A}+R_{A}\cdot R_{B}+R_{B}\cdot R_{C}}{R_{A}+R_{E}+R_{C}}\end{gathered}$$
### 三角形（Δ）到星形（Y）变换

$$R_{A}=\frac{R_{BC}\cdot R_{CA}}{R_{AB}+R_{BC}+R_{CA}}R_{B}=\frac{R_{CA}\cdot R_{AB}}{R_{AB}+R_{BC}+R_{CA}}R_{C}=\frac{R_{AB}\cdot R_{BC}}{R_{AB}+R_{BC}+R_{CA}}$$
